align better with paper

theories/simulang/simple_inv/examples/paper.v
@@ -1,11 +1,17 @@
 From simuliris.simulang Require Import lang notation tactics class_instances.
 From iris.proofmode Require Import tactics.
-From simuliris.simulation Require Import slsls lifting.
-From simuliris.simulang Require Import hoare.
-From simuliris.simulang.simple_inv Require Import inv.
+From simuliris.simulation Require Import slsls lifting .
+From simuliris.simulang Require Import hoare behavior.
+From simuliris.simulang.simple_inv Require Import inv adequacy.
 From iris.prelude Require Import options.
 
 (** * Examples from Section 2 of the paper *)
+(** Here, we prove both the quadruples shown in the paper,
+  and the logical relation (then deriving closed proofs of contextual refinement).
+
+  Normally, we would not bother with the quadruples, since the statement we are really
+   interested in is the contextual refinement.
+ *)
 
 Section fix_bi.
   Context `{!simpleGS Σ}.
@@ -23,14 +29,24 @@ Section fix_bi.
     sim_pures. source_load. sim_val. done.
   Qed.
 
+  (* for completeness : log_rel as described in Sec 4 *)
+  Lemma ex_2_1_log :
+    ⊢ log_rel ex_2_1_opt ex_2_1_unopt.
+  Proof.
+    log_rel. iModIntro. iIntros (π) "_".
+    source_alloc l_s as "Hl_s" "Hf_s".
+    target_alloc l_t as "Hl_t" "Hf_t".
+    sim_pures. source_load. sim_val. done.
+  Qed.
+
   (** First example from 2.2 *)
   Definition ex_2_2_1_unopt : expr :=
     let: "y" := ref(#42) in
-    Call f#"f" #42;;
+    Call f#"f" #23;;
     !"y".
   Definition ex_2_2_1_opt : expr :=
     let: "y" := ref(#42) in
-    Call f#"f" #42;;
+    Call f#"f" #23;;
     #42.
 
   Lemma ex_2_2_1 π :
@@ -45,6 +61,17 @@ Section fix_bi.
     source_load. sim_pures. sim_val. done.
   Qed.
 
+  Lemma ex_2_2_1_log :
+    ⊢ log_rel ex_2_2_1_opt ex_2_2_1_unopt.
+  Proof.
+    log_rel. iModIntro. iIntros (π) "_".
+    source_alloc l_s as "Hl_s" "Hf_s".
+    target_alloc l_t as "Hl_t" "Hf_t".
+    sim_pures.
+    sim_bind (Call _ _) (Call _ _). iApply sim_call; [done..|].
+    iIntros (??) "_". iApply lift_post_val.
+    source_load. sim_pures. sim_val. done.
+  Qed.
 
   (** Second example from 2.2 *)
   Definition ex_2_2_2_unopt : expr :=
@@ -62,6 +89,24 @@ Section fix_bi.
     ⊢ {{{ True }}} ex_2_2_2_opt ⪯[π] ex_2_2_2_unopt {{{ lift_post (λ v_t v_s, ⌜v_t = v_s⌝) }}}.
   Proof.
     iIntros "!> _". rewrite /ex_2_2_2_opt /ex_2_2_2_unopt.
+    source_alloc l_s as "Hl_s" "Hf_s".
+    target_alloc l_t as "Hl_t" "Hf_t".
+    source_load. sim_pures.
+    (* escape locations *)
+    iApply (sim_bij_insert with "Hf_t Hf_s Hl_t Hl_s []"); first done.
+    iIntros "#Hb".
+    sim_bind (Call _ _) (Call _ _). iApply sim_call; [done..|].
+    iIntros (??) "_". iApply lift_post_val.
+    sim_pures. sim_load v_t v_s as "Hv".
+    (* [omitted in the description in the paper] we use source UB to know that the loaded values must be integers *)
+    iApply sim_irred_unless. iIntros "[(%n & ->) _]".
+    val_discr_source "Hv". sim_pures. sim_val. done.
+  Qed.
+
+  Lemma ex_2_2_2_log :
+    ⊢ log_rel ex_2_2_2_opt ex_2_2_2_unopt.
+  Proof.
+    log_rel. iModIntro. iIntros (π) "_".
     source_alloc l_s as "Hl_s" "Hf_s".
     target_alloc l_t as "Hl_t" "Hf_t".
     source_load. sim_pures.
@@ -128,6 +173,40 @@ Section fix_bi.
     iIntros (??) "?". iApply lift_post_val. done.
   Qed.
 
+  Lemma ex_2_3_log :
+    ⊢ log_rel ex_2_3_opt ex_2_3_unopt.
+  Proof.
+    log_rel. iModIntro. iIntros (π) "_".
+    sim_bind (Call _ _) (Call _ _). iApply sim_call; [ done.. | ].
+    iIntros (p_t p_s) "Hv". iApply lift_post_val.
+    sim_pures.
+    source_bind (Fst _).
+    (* exploit source UB to know that the returned vlaue is a pair *)
+    iApply source_red_irred_unless. iIntros "(%x_s & %y_s & ->)".
+    iPoseProof (gen_val_rel_pair_source with "Hv") as "(%x_t & %y_t & -> & Hx_r & Hy_r)".
+    source_pures. sim_pures.
+    (* exploit source UB for the division *)
+    source_bind (_ `quot` _)%E.
+    iApply source_red_irred_unless. iIntros "[(%x & ->) (%y & -> & %Hy)]".
+    (* reduce the divisions *)
+    source_pure _.
+    { rewrite /bin_op_eval. simpl.
+      destruct (decide (y = 0%Z)) as [-> | _]; first done. reflexivity.
+    }
+    val_discr_source "Hx_r". val_discr_source "Hy_r".
+    target_pure _.
+    { rewrite /bin_op_eval. simpl.
+      destruct (decide (y = 0%Z)) as [-> | _]; first done. reflexivity.
+    }
+    simpl. generalize (Z.quot x y) => nz.
+    sim_pures.
+    (* use the gained knowledge *)
+    rewrite bool_decide_false; first last.
+    { contradict Hy. by simplify_eq. }
+    sim_pures. iApply sim_call; [ done.. | ].
+    iIntros (??) "H". iApply lift_post_val. iFrame.
+  Qed.
+
   (** Example from 2.4 *)
   Definition ex_2_4_unopt : expr :=
     let: "x" := ref(#0) in
@@ -183,5 +262,85 @@ Section fix_bi.
       iApply lift_post_val. done.
   Qed.
 
+  Lemma ex_2_4_log :
+    ⊢ log_rel ex_2_4_opt ex_2_4_unopt.
+  Proof.
+    log_rel. iModIntro. iIntros (π) "_".
+    source_alloc l_s as "Hl_s" "Hf_s".
+    target_alloc l_t as "Hl_t" "Hf_t".
+    target_load. sim_pures.
+
+    (* initiate coinduction with the following invariant:
+      (compared with the paper version, we carry through the right to deallocate,
+        for a more realistic example we might use that to deallocate the locations after
+        the loop)
+    *)
+    set inv := (†l_s…s 1 ∗ †l_t…t 1 ∗ l_s ↦s #0 ∗ l_t ↦t #0)%I.
+    iApply (sim_while_while _ _ _ _ _ inv with "[$Hf_s $Hl_s $Hf_t $Hl_t]").
+    iModIntro.
+    iIntros "(? & ? & Hl_s & Hl_t)".
+    (* loop condition *)
+    source_load.
+    sim_bind (Call _ _) (Call _ _).
+    iApply sim_call; [done..|].
+    iIntros (v_t v_s) "Hv". iApply lift_post_val.
+    (* retval must be bool *)
+    iApply sim_irred_unless. iIntros "(%b & ->)".
+    val_discr_source "Hv".
+
+    (* CA on loop condition *)
+    destruct b.
+    - (* true, do a loop iteration *)
+      sim_pures. source_load.
+      sim_bind (Call _ _) (Call _ _).
+      iApply sim_call;[done..|].
+      iIntros (??) "_"; iApply lift_post_val.
+      sim_pures.
+      (* use the coinduction hypothesis *)
+      iApply sim_expr_base.
+      iRight. iFrame. done.
+    - (* false, done with the loop *)
+      sim_pures. iApply sim_expr_base. iLeft.
+      iApply lift_post_val. done.
+  Qed.
+
 End fix_bi.
 
+
+Section closed.
+  (** Obtain a closed proof of [ctx_ref]. *)
+  Lemma ex_2_1_ctx : ctx_ref ex_2_1_opt ex_2_1_unopt.
+  Proof.
+    set Σ := #[simpleΣ].
+    apply (log_rel_adequacy Σ)=>?.
+    apply ex_2_1_log.
+  Qed.
+
+  Lemma ex_2_2_1_ctx : ctx_ref ex_2_2_1_opt ex_2_2_1_unopt.
+  Proof.
+    set Σ := #[simpleΣ].
+    apply (log_rel_adequacy Σ)=>?.
+    apply ex_2_2_1_log.
+  Qed.
+
+  Lemma ex_2_2_2_ctx : ctx_ref ex_2_2_2_opt ex_2_2_2_unopt.
+  Proof.
+    set Σ := #[simpleΣ].
+    apply (log_rel_adequacy Σ)=>?.
+    apply ex_2_2_2_log.
+  Qed.
+
+  Lemma ex_2_3_ctx : ctx_ref ex_2_3_opt ex_2_3_unopt.
+  Proof.
+    set Σ := #[simpleΣ].
+    apply (log_rel_adequacy Σ)=>?.
+    apply ex_2_3_log.
+  Qed.
+
+  Lemma ex_2_4_ctx : ctx_ref ex_2_4_opt ex_2_4_unopt.
+  Proof.
+    set Σ := #[simpleΣ].
+    apply (log_rel_adequacy Σ)=>?.
+    apply ex_2_4_log.
+  Qed.
+End closed.
